refinement proof in progress

memabs/CohRefine.v
@@ -1,2 +1,73 @@
-Require Import MemAbs.
+Require Import Relations RelationClasses.
+Require Import List.
+Require Import Integers Coqlib Maps.
+Require Import LanguageInterface Events Globalenvs Values Memory AST Errors Smallstep Linking.
+Require Import Clight Ctypes Cop SimplLocalsproof.
+Require Import CKLR Clightrel.
+Require Import Coherence CompCertSem Bigstep.
+Require Import SemDef.
 
+Section LTS.
+  Context {liA liB S} (L : lts liA liB S).
+
+  Inductive lts_ext_calls : S -> token (!liA) -> S -> Prop :=
+  | lts_ext_nil: forall s,
+      lts_ext_calls s nil s
+  | lts_ext_cons: forall s s' s'' q r t,
+      Smallstep.at_external L s q ->
+      Smallstep.after_external L s r s' ->
+      lts_ext_calls s' t s'' ->
+      lts_ext_calls s ((q, r) :: t) s''.
+
+  Lemma lts_trace_concat s s' t1 t2 r:
+    lts_ext_calls s t1 s' ->
+    lts_trace L false s' t2 r ->
+    lts_trace L false s (t1 ++ t2) r.
+  Proof.
+    intros H. induction H.
+    - auto.
+    - intros H'. specialize (IHlts_ext_calls H').
+      rewrite <- app_comm_cons. econstructor; eauto.
+      eapply lts_trace_steps. eapply Smallstep.star_refl. auto.
+  Qed.
+End LTS.
+
+(* So far I don't know how to prove this generally. Therefore, I think I will
+just add it to the DeepSEA correct criterion and it should be fairly
+straightforward for both getter/setter cases and abstract function cases *)
+Lemma trace_split {liA liB: language_interface} (σ: !liA --o !liB) q t r rest:
+  has σ (t, (q,r) :: rest) ->
+  exists t1 t2, t = t1 ++ t2 /\
+           exec σ q t1 r /\
+           has (next σ t1 q r) (t2, rest).
+(* Proof. *)
+(*   intros H. *)
+(*   assert (H': exists t', has σ (t', (q,r) :: nil)). *)
+
+Section REFINE.
+  Variable se: Genv.symtbl.
+  Variable C: Clight.program.
+  Variable Σ: Genv.symtbl -> !li_d --o !li_d.
+  (* li_dc is simply an adapter that forgets the memory in C calling
+  convertions *)
+  Let T1 := clight C se @ !li_dc @ (Σ se).
+  Let sk := AST.erase_program C.
+  (* Note that we can't prove the determinism of the mixed semantics. However we
+  should be able to prove the coherence when embed it into a linear function *)
+  Context (H : determinate (Abs.c_semantics sk C Σ)).
+  Let T2 := compcerto_lmap (Abs.c_semantics sk C Σ) H se.
+
+  Lemma mix_sem_ref: ref T1 T2.
+  Proof.
+    intros trace. cbn -[clight].
+    destruct trace as [bottom_tr top_tr].
+    intros (mid_tr_c & (mid_tr_d & Hbot & Hmid) & Htop).
+    destruct top_tr as [top_q top_r].
+    inversion Htop as [? s0 ? ? Hvq Hinit Htrace]. subst.
+    econstructor; [ apply Hvq | econstructor; apply Hinit | ].
+    clear Hvq Hinit Htop. clear T1 H T2.
+    revert mid_tr_d bottom_tr Σ Hmid Hbot.
+    induction Htrace.
+    admit. admit.
+
+  End REFINE.
